HoareLogic/Sound_Resource_TraceSemantics.v
@@ -1,0 +1,99 @@
+Require Import Coq.Logic.FunctionalExtensionality.
+Require Import Logic.lib.Coqlib.
+Require Import Logic.GeneralLogic.Base.
+Require Import Logic.MinimunLogic.Syntax.
+Require Import Logic.PropositionalLogic.Syntax.
+Require Import Logic.SeparationLogic.Syntax.
+Require Import Logic.GeneralLogic.KripkeModel.
+Require Import Logic.SeparationLogic.Model.SeparationAlgebra.
+Require Import Logic.PropositionalLogic.Semantics.Kripke.
+Require Import Logic.SeparationLogic.Semantics.FlatSemantics.
+Require Import Logic.HoareLogic.ImperativeLanguage.
+Require Import Logic.HoareLogic.ProgramState.
+Require Import Logic.HoareLogic.BigStepSemantics.
+Require Import Logic.HoareLogic.TraceSemantics.
+Require Import Logic.HoareLogic.HoareTriple_BigStepSemantics.
+Require Import Logic.HoareLogic.GuardedHoareTriple_TraceSemantics.
+
+Local Open Scope logic_base.
+Local Open Scope syntax.
+Local Open Scope kripke_model.
+Import PropositionalLanguageNotation.
+Import SeparationLogicNotation.
+Import KripkeModelSingleNotation.
+Import KripkeModelNotation_Intuitionistic.
+
+Section soundness.
+
+Existing Instance unit_kMD.
+
+Context {P: ProgrammingLanguage}
+        {MD: Model}
+        {J: Join model}
+        {R: Relation model}
+        {po_R: PreOrder Krelation}
+        {Res: Resource}
+        {Ac: Action}
+        {Acr: Action_resource Ac Res}
+        {TS: TraceSemantics P (model * resources) Ac}
+        {SAAIr: SAActionInterpret_resource model Ac Res ac_sem}.
+
+Context {L: Language} {nL: NormalLanguage L} {pL: PropositionalLanguage L} {SL: SeparationLanguage L} {SM: Semantics L MD} {kiSM: KripkeIntuitionisticSemantics L MD tt SM} {fsSM: FlatSemantics.SeparatingSemantics L MD tt SM}.
+
+Lemma hoare_parallel_partial_sound
+      {CPP: ConcurrentProgrammingLanguage_Sparallel P}
+      {AcP: Action_Parallel Ac}
+      {nAcPr: NormalAction_Parallel_resource Ac Res}
+      {c2tP: Command2Traces_Sparallel_resource P model Ac Res c2t}
+      {AIPr: ActionInterpret_Parallel_resource model Ac Res ac_sem}:
+  forall Inv c1 P1 Q1 c2 P2 Q2,
+  guarded_triple_partial_valid Inv P1 c1 Q1 ->
+  guarded_triple_partial_valid Inv P2 c2 Q2 ->
+  guarded_triple_partial_valid Inv (P1 * P2) (Sparallel c1 c2) (Q1 * Q2).
+Proof.
+  intros.
+  hnf in H, H0 |- *; intros.
+  unfold access, ThreadLocal_BSS in H, H0, H2; simpl in H, H0, H2.
+  inversion H2; subst; clear H2.
+  rewrite Sparallel_denote in H3.
+  set (Tr1 := cmd_denote c1) in H, H3.
+  set (Tr2 := cmd_denote c2) in H0, H3.
+  clearbody Tr1 Tr2; clear c1 c2.
+  inversion H3; subst; clear H3.
+  set (A1 := fun _: resource => False) in H at 1, H6 at 1.
+  set (A2 := fun _: resource => False) in H0 at 1, H6 at 1.
+  set (A := fun _: resource => False) in H4 at 1.
+  assert (forall r, A1 r \/ A2 r <-> A r) by (intro; subst A1 A2 A; simpl; tauto).
+  assert (forall r, A1 r -> A2 r -> False) by (intro; subst A1 A2; simpl; tauto).
+  clearbody A1 A2 A.
+  
+  rewrite sat_sepcon in H1.
+  destruct H1 as [s1 [s2 [? [? ?]]]].
+  specialize (fun ms_post HH => H s1 ms_post H8 (traces_access_intro tr1 _ _ _ H2 HH)).
+  specialize (fun ms_post HH => H0 s2 ms_post H9 (traces_access_intro tr2 _ _ _ H5 HH)).
+  clear Tr1 Tr2 H2 H5.
+  induction H6.
+  + inversion H4; subst; clear H4.
+    destruct ms_post; subst; inversion H2.
+    subst m A.
+    assert (A1 = fun _ => False) by (extensionality r; apply prop_ext; specialize (H3 r); tauto).
+    assert (A2 = fun _ => False) by (extensionality r; apply prop_ext; specialize (H3 r); tauto).
+    subst A1 A2.
+    specialize (H (Terminating s1) (trace_access_nil _)); simpl in H.
+    specialize (H0 (Terminating s2) (trace_access_nil _)); simpl in H0.
+    rewrite sat_sepcon.
+    exists s1, s2.
+    split; [| split]; auto.
+  + exfalso.
+    destruct (res_actions_no_race _ _ H2).
+    apply (state_enable_race_actions_spec a1 a2 A1 A2 s1 s2 s_pre); auto.
+    - intro.
+      rewrite (thread_local_state_enable_non_resource_action Inv) in H10 by auto.
+      specialize (H Error (@trace_access_Error _ _ (ThreadLocal_ActionInterpret_resource _ Inv) _ _ _ H10)).
+      inversion H.
+    - intro.
+      rewrite (thread_local_state_enable_non_resource_action Inv) in H10 by auto.
+      specialize (H0 Error (@trace_access_Error _ _ (ThreadLocal_ActionInterpret_resource _ Inv) _ _ _ H10)).
+      inversion H0.
+  + Abort.
+      
